dataplane/Examples/Ooo_Input_op.thy
@@ -8,8 +8,8 @@ begin
 record ('p, 'd, 'd1, 't) input_state = "('p, 'd, 'd1, 't) operator_state_ty" + es:: "'p \<Rightarrow> ('t, 'd1) event llist"
 
 definition ooo_input_op where
-  "ooo_input_op ops os = builder_op {||} ops os (\<lambda> os. (cimage (\<lambda>p. case es os p of
-    LNil \<Rightarrow> trace (STR ''Droping all'') (drop_caps os (map (\<lambda> t. Cap t p) (ocaps os p)))
+  "ooo_input_op ops os = builder_op False {||} ops os (\<lambda> os. (cimage (\<lambda>p. case es os p of
+    LNil \<Rightarrow> trace (STR ''Droping all: '' + show_nat (length (ocaps os p))) (drop_caps os (map (\<lambda> t. Cap t p) (ocaps os p)))
   | LCons (Data t d) lxs \<Rightarrow> produce (os\<lparr> es := (es os)(p := lxs) \<rparr>) (Cap t p) [en1 os d]
   | LCons (Drop t) lxs \<Rightarrow> drop_cap (os\<lparr> es := (es os)(p := lxs) \<rparr>) (Cap t p)
   | LCons (Mint t) lxs \<Rightarrow> add_cap (os\<lparr> es := (es os)(p := lxs) \<rparr>) p t)
@@ -26,7 +26,7 @@ definition input_ty_fun where
   | LCons (Mint t) lxs \<Rightarrow> mint_cap (ess_update (\<lambda> l. lxs) os) p t)"
 
 definition ooo_input_ty2_op where
-  "ooo_input_ty2_op os = builder_op {||} {|1 :: 2, 2|} os (\<lambda> os. (cimage (\<lambda>p.
+  "ooo_input_ty2_op os = builder_op False {||} {|1 :: 2, 2|} os (\<lambda> os. (cimage (\<lambda>p.
   (if p = 1 
   then
    input_ty_fun es1_update es1 os p
